test/artifact/lib/Hacl.Policies.fst
@@ -1,0 +1,53 @@
+module Hacl.Policies
+
+open FStar.ST
+open FStar.Buffer
+
+open Hacl.Types
+
+(* Module abbreviations *)
+module HS  = FStar.HyperStack
+module B   = FStar.Buffer
+module U8  = FStar.UInt8
+module U32 = FStar.UInt32
+module U64 = FStar.UInt64
+module H8  = Hacl.UInt8
+
+assume new type declassifiable (b:uint8_p)
+
+assume val leak_byte:
+  b:uint8_p ->
+  n:u32{U32.v n < length b} ->
+  Stack u8
+    (requires (fun h -> declassifiable b /\ live h b))
+    (ensures  (fun h0 z h1 -> live h0 b /\ h0 == h1 /\ U8.v z = H8.v (get h0 b (U32.v n))))
+
+
+val cmp_bytes_:
+  b:uint8_p{declassifiable b} ->
+  b':uint8_p{declassifiable b'} ->
+  len:u32{U32.v len <= length b /\ U32.v len <= length b'} ->
+  tmp:u8 ->
+  Stack u8
+    (requires (fun h -> live h b /\ live h b'))
+    (ensures  (fun h0 z h1 -> h0 == h1 /\ (U8.v z = 0 ==> as_seq h0 b == as_seq h0 b')))
+let rec cmp_bytes_ b b' len tmp =
+  if U32(len =^ 0ul) then U8.lognot tmp
+  else (
+    let i = U32 (len -^ 1ul) in
+    let bi = leak_byte b i in
+    let bi' = leak_byte b' i in
+    let tmp = U8 (eq_mask bi bi' &^ tmp) in
+    cmp_bytes_ b b' i tmp
+  )
+
+val cmp_bytes:
+  b:uint8_p{declassifiable b} ->
+  b':uint8_p{declassifiable b'} ->
+  len:u32{U32.v len <= length b /\ U32.v len <= length b'} ->
+  Stack u8
+    (requires (fun h -> live h b /\ live h b'))
+    (ensures  (fun h0 z h1 -> h0 == h1 /\ (U8.v z = 0 ==> as_seq h0 b == as_seq h0 b')))
+let cmp_bytes b b' len =
+  cmp_bytes_ b b' len 255uy
+
