test/artifact/pneutube/crypto/Hacl.EC.Curve25519.Bignum.Fdifference.fst
@@ -1,0 +1,92 @@
+module Hacl.EC.Curve25519.Bignum.Fdifference
+
+open FStar.Mul
+open FStar.ST
+open FStar.HyperStack
+open FStar.Ghost
+open FStar.Buffer
+open FStar.Math.Lib
+
+open Hacl.UInt64
+
+open Hacl.EC.Curve25519.Parameters
+open Hacl.EC.Curve25519.Bigint
+open Hacl.EC.Curve25519.Utils
+
+#reset-options "--initial_fuel 0 --max_fuel 0"
+
+(* Module abbreviations *)
+module HH = FStar.HyperHeap
+module HS = FStar.HyperStack
+
+module U8  = FStar.UInt8
+module U32 = FStar.UInt32
+module H8  = Hacl.UInt8
+module H32  = Hacl.UInt32
+module H64  = Hacl.UInt64
+
+#reset-options "--initial_fuel 0 --max_fuel 0"
+
+val add_big_zero_:
+  b:bigint ->
+  Stack unit
+    (requires (fun h -> live h b))
+    (ensures (fun h0 _ h1 -> live h1 b /\ modifies_1 b h0 h1))
+let add_big_zero_ b =
+  let two52m38 = (Hacl.Cast.uint64_to_sint64 0xfffffffffffdauL) in // pow2 52 - 38
+  let two52m2 =  (Hacl.Cast.uint64_to_sint64 0xffffffffffffeuL) in // pow2 52 - 2
+  let b0 = b.(0ul) in
+  let b1 = b.(1ul) in
+  let b2 = b.(2ul) in
+  let b3 = b.(3ul) in
+  let b4 = b.(4ul) in
+  let c0 = b0 +%^ two52m38 in
+  let c1 = b1 +%^ two52m2  in
+  let c2 = b2 +%^ two52m2  in
+  let c3 = b3 +%^ two52m2  in
+  let c4 = b4 +%^ two52m2  in
+  update_5 b c0 c1 c2 c3 c4
+
+
+val add_big_zero:
+  b:bigint ->
+  Stack unit
+    (requires (fun h -> live h b))
+    (ensures (fun h0 _ h1 -> live h1 b /\ modifies_1 b h0 h1))
+let add_big_zero b =
+  add_big_zero_ b
+
+
+val fdifference_:
+  a:bigint ->
+  b:bigint{disjoint a b} ->
+  Stack unit
+    (requires (fun h -> live h a /\ live h b))
+    (ensures (fun h0 _ h1 -> live h1 a /\ modifies_1 a h0 h1))
+let fdifference_ a b =
+  let a0 = a.(0ul) in
+  let a1 = a.(1ul) in
+  let a2 = a.(2ul) in
+  let a3 = a.(3ul) in
+  let a4 = a.(4ul) in
+  let b0 = b.(0ul) in
+  let b1 = b.(1ul) in
+  let b2 = b.(2ul) in
+  let b3 = b.(3ul) in
+  let b4 = b.(4ul) in
+  let c0 = b0 -%^ a0 in
+  let c1 = b1 -%^ a1 in
+  let c2 = b2 -%^ a2 in
+  let c3 = b3 -%^ a3 in
+  let c4 = b4 -%^ a4 in
+  update_5 a c0 c1 c2 c3 c4
+
+
+val fdifference':
+  a:bigint ->
+  b:bigint{disjoint a b} ->
+  Stack unit
+    (requires (fun h -> live h a /\ live h b))
+    (ensures (fun h0 u h1 -> live h1 a /\ modifies_1 a h0 h1))
+let fdifference' a b =
+  fdifference_ a b
