test/artifact/pneutube/crypto/Hacl.EC.Curve25519.Bignum.Fproduct.fst
@@ -1,0 +1,100 @@
+module Hacl.EC.Curve25519.Bignum.Fproduct
+
+open FStar.Mul
+open FStar.ST
+open FStar.HyperStack
+open FStar.Ghost
+open FStar.Math.Lib
+open FStar.Math.Lemmas
+open FStar.Buffer
+open FStar.Buffer.Quantifiers
+
+open Hacl.UInt64
+
+open Hacl.EC.Curve25519.Parameters
+open Hacl.EC.Curve25519.Bigint
+open Hacl.EC.Curve25519.Utils
+
+#reset-options "--initial_fuel 0 --max_fuel 0"
+
+(* Module abbreviations *)
+module HH = FStar.HyperHeap
+module HS = FStar.HyperStack
+
+module U8  = FStar.UInt8
+module U32 = FStar.UInt32
+module H8  = Hacl.UInt8
+module H32  = Hacl.UInt32
+module H64  = Hacl.UInt64
+module H128  = Hacl.UInt128
+
+private val multiplication_0:
+  c:bigint_wide{length c >= 2*norm_length-1} ->
+  a0:H64.t -> a1:H64.t -> a2:H64.t -> a3:H64.t -> a4:H64.t ->
+  b0:H64.t -> b1:H64.t -> b2:H64.t -> b3:H64.t -> b4:H64.t ->
+  Stack unit
+    (requires (fun h -> live h c))
+    (ensures  (fun h0 _ h1 -> modifies_1 c h0 h1 /\ live h1 c))
+let multiplication_0 c a0 a1 a2 a3 a4 b0 b1 b2 b3 b4 =
+  let open Hacl.UInt128 in
+  let ab00 = a0 *^ b0 in
+  let ab01 = a0 *^ b1 in
+  let ab02 = a0 *^ b2 in
+  let ab03 = a0 *^ b3 in
+  let ab04 = a0 *^ b4 in
+  let ab10 = a1 *^ b0 in
+  let ab11 = a1 *^ b1 in
+  let ab12 = a1 *^ b2 in
+  let ab13 = a1 *^ b3 in
+  let ab14 = a1 *^ b4 in
+  let ab20 = a2 *^ b0 in
+  let ab21 = a2 *^ b1 in
+  let ab22 = a2 *^ b2 in
+  let ab23 = a2 *^ b3 in
+  let ab24 = a2 *^ b4 in
+  let ab30 = a3 *^ b0 in
+  let ab31 = a3 *^ b1 in
+  let ab32 = a3 *^ b2 in
+  let ab33 = a3 *^ b3 in
+  let ab34 = a3 *^ b4 in
+  let ab40 = a4 *^ b0 in
+  let ab41 = a4 *^ b1 in
+  let ab42 = a4 *^ b2 in
+  let ab43 = a4 *^ b3 in
+  let ab44 = a4 *^ b4 in
+  let open Hacl.UInt64 in
+  let c0 = ab00 in
+  let c1 = H128 (ab01 +%^ ab10) in
+  let c2 = H128 (ab02 +%^ ab11 +%^ ab20) in
+  let c3 = H128 (ab03 +%^ ab12 +%^ ab21 +%^ ab30) in
+  let c4 = H128 (ab04 +%^ ab13 +%^ ab22 +%^ ab31 +%^ ab40) in
+  let c5 = H128 (ab14 +%^ ab23 +%^ ab32 +%^ ab41) in
+  let c6 = H128 (ab24 +%^ ab33 +%^ ab42) in
+  let c7 = H128 (ab34 +%^ ab43) in
+  let c8 = ab44 in
+  update_wide_9 c c0 c1 c2 c3 c4 c5 c6 c7 c8
+
+
+private val multiplication_:
+  c:bigint_wide{length c >= 2 * norm_length - 1} ->
+  a:bigint{disjoint c a} ->
+  b:bigint{disjoint c b} ->
+  Stack unit
+     (requires (fun h -> live h a /\ live h b /\ live h c))
+     (ensures (fun h0 u h1 -> live h1 c /\ modifies_1 c h0 h1))
+let multiplication_ c a b =
+  let h0 = ST.get() in
+  let a0 = a.(0ul) in let a1 = a.(1ul) in let a2 = a.(2ul) in let a3 = a.(3ul) in let a4 = a.(4ul) in
+  let b0 = b.(0ul) in let b1 = b.(1ul) in let b2 = b.(2ul) in let b3 = b.(3ul) in let b4 = b.(4ul) in
+  multiplication_0 c a0 a1 a2 a3 a4 b0 b1 b2 b3 b4
+
+
+val multiplication:
+  c:bigint_wide{length c >= 2 * norm_length - 1} ->
+  a:bigint{disjoint c a} ->
+  b:bigint{disjoint c b} ->
+  Stack unit
+     (requires (fun h -> live h a /\ live h b /\ live h c))
+     (ensures (fun h0 u h1 -> live h1 c /\ modifies_1 c h0 h1))
+let multiplication c a b =
+  multiplication_ c a b
