test/artifact/pneutube/crypto/Hacl.EC.Curve25519.Bignum.Fscalar.fst
@@ -1,0 +1,56 @@
+module Hacl.EC.Curve25519.Bignum.Fscalar
+
+open FStar.Mul
+open FStar.ST
+open FStar.HyperStack
+open FStar.Buffer
+open FStar.Buffer.Quantifiers
+(* open Hacl.SBuffer *)
+open FStar.Math.Lib
+open FStar.Ghost
+open Hacl.UInt64
+
+open Hacl.EC.Curve25519.Parameters
+open Hacl.EC.Curve25519.Bigint
+open Hacl.EC.Curve25519.Utils
+
+#reset-options "--initial_fuel 0 --max_fuel 0"
+
+(* Module abbreviations *)
+module HH = FStar.HyperHeap
+module HS = FStar.HyperStack
+
+module U8  = FStar.UInt8
+module U32 = FStar.UInt32
+module H8  = Hacl.UInt8
+module H32  = Hacl.UInt32
+module H64  = Hacl.UInt64
+
+
+val fscalar_:
+  res:bigint_wide ->
+  a:bigint{disjoint res a} ->
+  s:s64 ->
+  Stack unit
+    (requires (fun h -> live h res /\ live h a))
+    (ensures (fun h0 _ h1 -> live h1 res /\ modifies_1 res h0 h1))
+let fscalar_ res a s =
+  let a0 = a.(0ul) in
+  let a1 = a.(1ul) in
+  let a2 = a.(2ul) in
+  let a3 = a.(3ul) in
+  let a4 = a.(4ul) in
+  let open Hacl.UInt128 in
+  let r0 = a0 *^ s in
+  let r1 = a1 *^ s in
+  let r2 = a2 *^ s in
+  let r3 = a3 *^ s in
+  let r4 = a4 *^ s in
+  update_wide_5 res r0 r1 r2 r3 r4
+
+
+val scalar': res:bigint_wide -> a:bigint{disjoint res a} -> s:s64 -> STL unit
+     (requires (fun h -> live h a /\ live h res))
+     (ensures (fun h0 u h1 -> live h1 res /\ modifies_1 res h0 h1))
+let scalar' res a s =
+  fscalar_ res a s
