test/artifact/pneutube/crypto/Hacl.EC.Curve25519.Bignum.Fsum.fst
@@ -1,0 +1,66 @@
+module Hacl.EC.Curve25519.Bignum.Fsum
+
+open FStar.Mul
+open FStar.ST
+open FStar.HyperStack
+open FStar.Buffer
+open FStar.Buffer.Quantifiers
+(* open Hacl.SBuffer *)
+open FStar.Math.Lib
+open FStar.Ghost
+open Hacl.UInt64
+
+open Hacl.EC.Curve25519.Parameters
+open Hacl.EC.Curve25519.Bigint
+open Hacl.EC.Curve25519.Utils
+
+#reset-options "--initial_fuel 0 --max_fuel 0"
+
+(* Module abbreviations *)
+module HH = FStar.HyperHeap
+module HS = FStar.HyperStack
+
+module U8  = FStar.UInt8
+module U32 = FStar.UInt32
+module H8  = Hacl.UInt8
+module H32  = Hacl.UInt32
+module H64  = Hacl.UInt64
+
+private val fsum_:
+  a:bigint ->
+  b:bigint{disjoint a b} ->
+  Stack unit
+    (requires (fun h -> live h a /\ live h b))
+    (ensures (fun h0 u h1 -> live h1 a /\ modifies_1 a h0 h1))
+let fsum_ a b =
+  let h0 = ST.get() in
+  let a0 = a.(0ul) in
+  let a1 = a.(1ul) in
+  let a2 = a.(2ul) in
+  let a3 = a.(3ul) in
+  let a4 = a.(4ul) in
+  let b0 = b.(0ul) in
+  let b1 = b.(1ul) in
+  let b2 = b.(2ul) in
+  let b3 = b.(3ul) in
+  let b4 = b.(4ul) in
+  assert(v a0 = v (get h0 a 0)); assert(v a1 = v (get h0 a 1)); assert(v a2 = v (get h0 a 2));
+  assert(v a3 = v (get h0 a 3)); assert(v a4 = v (get h0 a 4)); assert(v b0 = v (get h0 b 0));
+  assert(v b1 = v (get h0 b 1)); assert(v b2 = v (get h0 b 2)); assert(v b3 = v (get h0 b 3));
+  assert(v b4 = v (get h0 b 4));
+  let ab0 = a0 +%^ b0 in
+  let ab1 = a1 +%^ b1 in
+  let ab2 = a2 +%^ b2 in
+  let ab3 = a3 +%^ b3 in
+  let ab4 = a4 +%^ b4 in
+  update_5 a ab0 ab1 ab2 ab3 ab4
+
+
+val fsum':
+  a:bigint ->
+  b:bigint{disjoint a b} ->
+  Stack unit
+    (requires (fun h -> live h a /\ live h b))
+    (ensures (fun h0 u h1 -> live h1 a /\ modifies_1 a h0 h1))
+let fsum' a b =
+  fsum_ a b
