test/artifact/pneutube/crypto/Hacl.EC.Curve25519.Bignum.fst
@@ -1,0 +1,158 @@
+module Hacl.EC.Curve25519.Bignum
+
+open FStar.Mul
+open FStar.ST
+open FStar.HyperStack
+open FStar.Ghost
+open Hacl.UInt64
+
+open FStar.Buffer
+open FStar.Math.Lib
+open Hacl.EC.Curve25519.Parameters
+open Hacl.EC.Curve25519.Bigint
+open Hacl.EC.Curve25519.Utils
+
+#reset-options "--initial_fuel 0 --max_fuel 0 --z3timeout 20"
+
+
+(* Module abbreviations *)
+module HH = FStar.HyperHeap
+module HS = FStar.HyperStack
+
+module U8  = FStar.UInt8
+module U32 = FStar.UInt32
+module H8  = Hacl.UInt8
+module H32  = Hacl.UInt32
+module H64  = Hacl.UInt64
+module H128  = Hacl.UInt128
+
+
+val copy_bigint: output:bigint -> input:bigint{disjoint input output} -> Stack unit
+  (requires (fun h -> live h output /\ live h input))
+  (ensures  (fun h0 _ h1 -> live h1 output /\ modifies_1 output h0 h1))
+let copy_bigint output i =
+  let i0 = i.(0ul) in
+  let i1 = i.(1ul) in
+  let i2 = i.(2ul) in
+  let i3 = i.(3ul) in
+  let i4 = i.(4ul) in
+  update_5 output i0 i1 i2 i3 i4
+
+
+val copy_to_bigint': output:bigint -> input:bigint_wide{disjoint input output} -> Stack unit
+    (requires (fun h -> live h output /\ live h input))
+    (ensures (fun h0 _ h1 -> live h1 output /\ modifies_1 output h0 h1))
+let rec copy_to_bigint' output b =
+  Math.Lemmas.pow2_lt_compat 128 64;
+  let b0 = b.(0ul) in
+  let b1 = b.(1ul) in
+  let b2 = b.(2ul) in
+  let b3 = b.(3ul) in
+  let b4 = b.(4ul) in
+  let open Hacl.UInt128 in
+  update_5 output (Hacl.Cast.sint128_to_sint64 b0)
+                 (Hacl.Cast.sint128_to_sint64 b1)
+                 (Hacl.Cast.sint128_to_sint64 b2)
+                 (Hacl.Cast.sint128_to_sint64 b3)
+                 (Hacl.Cast.sint128_to_sint64 b4)
+
+
+val copy_to_bigint:
+  output:bigint ->
+  input:bigint_wide{disjoint input output} ->
+  Stack unit
+    (requires (fun h -> live h output /\ live h input))
+    (ensures (fun h0 _ h1 -> modifies_1 output h0 h1 /\ live h1 output))
+let copy_to_bigint output b =
+  copy_to_bigint' output b
+
+
+val copy_to_bigint_wide': output:bigint_wide -> input:bigint{disjoint input output} -> Stack unit
+    (requires (fun h -> live h output /\ live h input))
+    (ensures (fun h0 _ h1 -> live h1 output /\ modifies_1 output h0 h1))
+let rec copy_to_bigint_wide' output b =
+  let b0 = b.(0ul) in
+  let b1 = b.(1ul) in
+  let b2 = b.(2ul) in
+  let b3 = b.(3ul) in
+  let b4 = b.(4ul) in
+  update_wide_5 output (Hacl.Cast.sint64_to_sint128 b0)
+                      (Hacl.Cast.sint64_to_sint128 b1)
+                      (Hacl.Cast.sint64_to_sint128 b2)
+                      (Hacl.Cast.sint64_to_sint128 b3)
+                      (Hacl.Cast.sint64_to_sint128 b4)
+
+
+val copy_to_bigint_wide: output:bigint_wide -> input:bigint{disjoint input output} -> Stack unit
+    (requires (fun h -> live h output /\ live h input))
+    (ensures (fun h0 _ h1 -> live h1 output /\ modifies_1 output h0 h1))
+let copy_to_bigint_wide output b =
+  copy_to_bigint_wide' output b
+
+
+val modulo:
+  output:bigint ->
+  input:bigint_wide{disjoint input output} ->
+  Stack unit
+    (requires (fun h -> live h input /\ live h output /\ length input >= 2*norm_length - 1 ))
+    (ensures (fun h0 _ h1 -> live h1 output /\ live h1 input /\ modifies_2 output input h0 h1))
+let modulo output b =
+  Hacl.EC.Curve25519.Bignum.Modulo.freduce_degree b;
+  Hacl.EC.Curve25519.Bignum.Modulo.freduce_coefficients_wide b;
+  copy_to_bigint output b
+
+
+val fsum: a:bigint{length a >= norm_length + 1} -> b:bigint{disjoint a b} -> Stack unit
+    (requires (fun h -> live h a /\ live h b))
+    (ensures (fun h0 _ h1 -> live h1 a /\ modifies_1 a h0 h1))
+let fsum a b =
+  Hacl.EC.Curve25519.Bignum.Fsum.fsum' a b;
+  Hacl.EC.Curve25519.Bignum.Modulo.freduce_coefficients a
+
+
+#reset-options "--z3timeout 20 --initial_fuel 0 --max_fuel 0"
+
+val fdifference: a:bigint{length a >= norm_length+1} -> b:bigint{disjoint a b} -> Stack unit
+    (requires (fun h -> live h a /\ live h b))
+    (ensures (fun h0 _ h1 -> live h1 a /\ modifies_1 a h0 h1))
+let fdifference a b =
+  push_frame ();
+  let b' = create (Hacl.Cast.uint64_to_sint64 0uL) nlength in
+  copy_bigint b' b;
+  Hacl.EC.Curve25519.Bignum.Fdifference.add_big_zero b';
+  Hacl.EC.Curve25519.Bignum.Fdifference.fdifference' a b';
+  Hacl.EC.Curve25519.Bignum.Modulo.freduce_coefficients a;
+  pop_frame()
+
+
+#reset-options "--z3timeout 20 --initial_fuel 0 --max_fuel 0"
+
+val fscalar:
+    res:bigint -> b:bigint{disjoint res b} -> s:s64 -> Stack unit
+  (requires (fun h -> live h res /\ live h b))
+  (ensures (fun h0 _ h1 -> live h1 res /\ modifies_1 res h0 h1))
+let fscalar res b s =
+  push_frame ();
+  let tmp = create (Hacl.Cast.uint64_to_sint128 0uL) (6ul) in
+  Hacl.EC.Curve25519.Bignum.Fscalar.scalar' tmp b s;
+  Hacl.EC.Curve25519.Bignum.Modulo.freduce_coefficients_wide tmp;
+  copy_to_bigint res tmp;
+  pop_frame()
+
+
+val fmul: res:bigint -> a:bigint{disjoint res a} -> b:bigint{disjoint res b} -> Stack unit
+    (requires (fun h -> live h res /\ live h a /\ live h b))
+    (ensures (fun h0 _ h1 -> live h1 res /\ modifies_1 res h0 h1))
+let fmul res a b =
+  push_frame ();
+  let tmp = create (Hacl.Cast.uint64_to_sint128 0uL) 9ul in
+  Hacl.EC.Curve25519.Bignum.Fproduct.multiplication tmp a b;
+  modulo res tmp;
+  pop_frame()
+
+
+val fsquare: res:bigint -> a:bigint{disjoint res a} -> Stack unit
+    (requires (fun h -> live h res /\ live h a))
+    (ensures (fun h0 _ h1 -> live h1 res /\ modifies_1 res h0 h1))
+let fsquare res a =
+  fmul res a a
