test/artifact/pneutube/crypto/Hacl.EC.Curve25519.PPoint.fst
@@ -1,0 +1,363 @@
+module Hacl.EC.Curve25519.PPoint
+
+open FStar.Mul
+open FStar.ST
+open FStar.HyperStack
+open FStar.Ghost
+open FStar.Buffer
+open Hacl.UInt64
+
+open FStar.Buffer
+open FStar.Math.Lib
+open Hacl.EC.Curve25519.Parameters
+open Hacl.EC.Curve25519.Bigint
+open Hacl.EC.Curve25519.Bignum
+
+
+#reset-options "--initial_fuel 0 --max_fuel 0"
+
+(* Module abbreviations *)
+module B  = FStar.Buffer
+module HH = FStar.HyperHeap
+module HS = FStar.HyperStack
+
+module U8  = FStar.UInt8
+module U32 = FStar.UInt32
+module H8  = Hacl.UInt8
+module H32  = Hacl.UInt32
+module H64  = Hacl.UInt64
+module H128  = Hacl.UInt128
+
+
+noeq type point =
+  | Point: x:bigint{length x = 6} ->
+           y:bigint ->
+           z:bigint{length z = 6} ->
+           point
+
+
+val get_x: point -> Tot bigint
+let get_x p = Point.x p
+val get_y: point -> Tot bigint
+let get_y p = Point.y p
+val get_z: point -> Tot bigint
+let get_z p = Point.z p
+
+
+val make: x:bigint{length x = 6} -> bigint -> z:bigint{length z = 6} -> Tot point
+let make x y z = Point x y z
+
+
+// Separation between the references of all three coordinates
+type separateCoordinates (p:point) =
+  disjoint (get_x p) (get_y p) /\ disjoint (get_x p) (get_z p) /\ disjoint (get_y p) (get_z p)
+
+
+// Point "live" in memory 'h'
+type live (h:heap) (p:point) =
+  live h (get_x p) /\ live h (get_y p) /\ live h (get_z p) /\ separateCoordinates p
+
+
+// Two distincts points from a memory point of view
+type distinct (a:point) (b:point) =
+  disjoint (get_x a) (get_x b) /\ disjoint (get_x a) (get_y b) /\ disjoint (get_x a) (get_z b)
+  /\ disjoint (get_y a) (get_x b) /\ disjoint (get_y a) (get_y b) /\ disjoint (get_y a) (get_z b)
+  /\ disjoint (get_z a) (get_x b) /\ disjoint (get_z a) (get_y b) /\ disjoint (get_z a) (get_z b)
+
+
+let op_Plus_Plus (#a:Type) (s:TSet.set a) (s':TSet.set a) : GTot (TSet.set a) = TSet.union s s'
+
+
+val refs: p:point -> GTot (TSet.set Heap.aref)
+let refs p = arefs (only (get_x p) ++ only (get_y p) ++ (only (get_z p)))
+
+
+val swap_conditional_aux': a:bigint -> b:bigint{disjoint a b} ->
+  is_swap:s64 ->
+  ctr:u32{U32.v ctr<=norm_length} -> STL unit
+    (requires (fun h -> B.live h a /\ B.live h b))
+    (ensures (fun h0 _ h1 -> B.live h1 a /\ B.live h1 b /\ modifies_2 a b h0 h1))
+let rec swap_conditional_aux' a b swap ctr =
+  if U32 (nlength =^ ctr) then ()
+  else begin
+    let ai = a.(ctr) in
+    let bi = b.(ctr) in
+    let y = ai ^^ bi in
+    let x = swap &^ y in
+    let ai' =  x ^^ ai in
+    let bi' = x ^^ bi in
+    a.(ctr) <- ai';
+    b.(ctr) <- bi';
+    swap_conditional_aux' a b swap (U32 (ctr +^ 1ul));
+    ()
+ end
+
+val swap_conditional_aux: a:bigint -> b:bigint{disjoint a b} ->
+  is_swap:s64 ->
+  Stack unit
+    (requires (fun h -> B.live h a /\ B.live h b))
+    (ensures (fun h0 _ h1 -> B.live h1 a /\ B.live h1 b /\ modifies_2 a b h0 h1))
+let rec swap_conditional_aux a b swap =
+  swap_conditional_aux' a b swap 0ul
+
+
+#reset-options "--initial_fuel 0 --max_fuel 0 --z3timeout 5"
+
+(* For simplicity, assuming that the point coordinates have been allocated on the same frame.
+   Ideally in the same buffer *)
+type same_frame (p:point) =
+  frameOf (get_x p) = frameOf (get_y p) /\ frameOf (get_x p) = frameOf (get_z p)
+type same_frame_2 (p:point) (p':point) =
+  same_frame p /\ same_frame p' /\ frameOf (get_x p) = frameOf (get_x p')
+
+
+let frame_of (p:point{same_frame p}) : GTot HH.rid = frameOf (get_x p)
+
+val helper_lemma: #t:Type -> a:buffer t -> b:buffer t -> Lemma
+  (requires (True))
+  (ensures  (arefs (only a ++ only b) == !{as_ref a, as_ref b}))
+let helper_lemma #t a b =
+  let s =  only a ++ only b in
+  let s' = !{as_ref a, as_ref b} in
+  assert(TSet.mem (Buff a) s);
+  assert(TSet.mem (Buff b) s);
+  TSet.lemma_equal_intro (arefs s) s'
+
+
+let helper_lemma_2 r h0 h1 (sub:TSet.set Heap.aref) (s:TSet.set Heap.aref) : Lemma
+  (requires (TSet.subset sub s /\ modifies_ref r sub h0 h1))
+  (ensures  (modifies_ref r s h0 h1))
+  = ()
+
+
+let helper_lemma_3 r h0 h1 h2 s : Lemma
+  (requires (HS.modifies_ref r s h0 h1 /\ HS.modifies_ref r s h1 h2))
+  (ensures  (HS.modifies_ref r s h0 h2))
+  = ()
+
+let prop_1 h0 h1 (a:point) (b:point) : GTot Type0 =
+  same_frame_2 a b
+  /\ (forall (#t:Type) (b':buffer t). (frameOf b' = frame_of a /\ B.live h0 b'
+       /\ disjoint_from_bufs b' (only (get_x a) ++ only (get_y a) ++ only (get_z a)
+				    ++ only (get_x b) ++ only (get_y b) ++ only (get_z b) ))
+				    ==> equal h0 b' h1 b')
+
+#reset-options "--initial_fuel 0 --max_fuel 0 --z3timeout 20"
+
+let helper_lemma_4 r h0 h1 h2 h3 a b : Lemma
+  (requires ( (forall (#t:Type) (b':buffer t). (frameOf b' = frame_of a /\ B.live h0 b'
+      /\ disjoint b' (get_x a) /\ disjoint b' (get_x b))  ==> equal h0 b' h1 b')
+    /\ (forall (#t:Type) (b':buffer t). (frameOf b' = frame_of a /\ B.live h1 b'
+      /\ disjoint b' (get_y a) /\ disjoint b' (get_y b))  ==> equal h1 b' h2 b')
+    /\ (forall (#t:Type) (b':buffer t). (frameOf b' = frame_of a /\ B.live h2 b'
+      /\ disjoint b' (get_z a) /\ disjoint b' (get_z b))  ==> equal h2 b' h3 b')
+     /\ same_frame_2 a b ))
+   (ensures  (prop_1 h0 h3 a b))
+  = let s = only (get_x a) ++ only (get_y a) ++ only (get_z a)
+	    ++ only (get_x b) ++ only (get_y b) ++ only (get_z b) in
+    assert(TSet.mem (Buff (get_x a)) s);
+    assert(TSet.mem (Buff (get_y a)) s);
+    assert(TSet.mem (Buff (get_z a)) s);
+    assert(TSet.mem (Buff (get_x b)) s);
+    assert(TSet.mem (Buff (get_y b)) s);
+    assert(TSet.mem (Buff (get_z b)) s);
+    assert(forall (#t:Type) (b':buffer t). disjoint_from_bufs b' s
+	     ==> (disjoint b' (get_x a) /\ disjoint b' (get_x b)));
+    assert(forall (#t:Type) (b':buffer t). disjoint_from_bufs b' s
+	     ==> (disjoint b' (get_y a) /\ disjoint b' (get_y b)));
+    assert(forall (#t:Type) (b':buffer t). disjoint_from_bufs b' s
+	     ==> (disjoint b' (get_z a) /\ disjoint b' (get_z b)))
+
+
+#reset-options "--initial_fuel 0 --max_fuel 0 --z3timeout 100"
+
+val swap_conditional:
+  a:point{same_frame a} -> b:point{distinct a b /\ same_frame b} ->
+  is_swap:s64 ->
+  Stack unit
+    (requires (fun h -> live h a /\ live h b /\ same_frame_2 a b))
+    (ensures (fun h0 _ h1 -> live h1 a /\ live h1 b
+      /\ HS.modifies_one (frame_of a) h0 h1
+      /\ HS.modifies_ref (frame_of a) (refs a ++ refs b) h0 h1
+      /\ prop_1 h0 h1 a b))
+let swap_conditional a b is_swap =
+  let h0 = ST.get() in
+  swap_conditional_aux (get_x a) (get_x b) is_swap;
+  let h1 = ST.get() in
+  lemma_reveal_modifies_2 (get_x a) (get_x b) h0 h1;
+  cut (live h1 a /\ live h1 b);
+  swap_conditional_aux (get_y a) (get_y b) is_swap;
+  let h2 = ST.get() in
+  cut (live h2 a /\ live h2 b);
+  lemma_reveal_modifies_2 (get_y a) (get_y b) h1 h2;
+  swap_conditional_aux (get_z a) (get_z b) is_swap;
+  let h3 = ST.get() in
+  cut (live h3 a /\ live h3 b);
+  lemma_reveal_modifies_2 (get_z a) (get_z b) h2 h3;
+  assert(HS.modifies_one (frame_of a) h0 h3);
+  helper_lemma (get_x a) (get_x b);
+  helper_lemma (get_y a) (get_y b);
+  helper_lemma (get_z a) (get_z b);
+  helper_lemma_2 (frame_of a) h0 h1 !{as_ref (get_x a), as_ref (get_x b)} (refs a ++ refs b);
+  helper_lemma_2 (frame_of a) h1 h2 !{as_ref (get_y a), as_ref (get_y b)} (refs a ++ refs b);
+  helper_lemma_2 (frame_of a) h2 h3 !{as_ref (get_z a), as_ref (get_z b)} (refs a ++ refs b);
+  helper_lemma_3 (frame_of a) h0 h1 h2 (refs a ++ refs b);
+  helper_lemma_3 (frame_of a) h0 h2 h3 (refs a ++ refs b);
+  helper_lemma_4 (frame_of a) h0 h1 h2 h3 a b;
+  assert(HS.modifies_ref (frame_of a) (refs a ++ refs b) h0 h3);
+  ()
+
+
+#reset-options "--initial_fuel 0 --max_fuel 0 --z3timeout 20"
+
+val helper_lemma': #t:Type -> a:buffer t -> Lemma
+  (requires (True))
+  (ensures  (arefs (only a) == !{as_ref a}))
+let helper_lemma' #t a =
+  let s =  only a in
+  let s' = !{as_ref a} in
+  assert(TSet.mem (Buff a) s);
+  TSet.lemma_equal_intro (arefs s) s'
+
+let prop_2 h0 h1 (a:point) : GTot Type0 =
+  same_frame a
+  /\ (forall (#t:Type) (b':buffer t). (frameOf b' = frame_of a /\ B.live h0 b'
+       /\ disjoint_from_bufs b' (only (get_x a) ++ only (get_y a) ++ only (get_z a)))
+				    ==> equal h0 b' h1 b')
+
+let helper_lemma_4' r h0 h1 h2 h3 a : Lemma
+  (requires ( (forall (#t:Type) (b':buffer t). (frameOf b' = frame_of a /\ B.live h0 b'
+      /\ disjoint b' (get_x a))  ==> equal h0 b' h1 b')
+    /\ (forall (#t:Type) (b':buffer t). (frameOf b' = frame_of a /\ B.live h1 b'
+      /\ disjoint b' (get_y a))  ==> equal h1 b' h2 b')
+    /\ (forall (#t:Type) (b':buffer t). (frameOf b' = frame_of a /\ B.live h2 b'
+      /\ disjoint b' (get_z a))  ==> equal h2 b' h3 b')
+     /\ same_frame a ))
+   (ensures  (prop_2 h0 h3 a))
+  = let s = only (get_x a) ++ only (get_y a) ++ only (get_z a) in
+    assert(TSet.mem (Buff (get_x a)) s);
+    assert(TSet.mem (Buff (get_y a)) s);
+    assert(TSet.mem (Buff (get_z a)) s);
+    assert(forall (#t:Type) (b':buffer t). disjoint_from_bufs b' s
+	     ==> (disjoint b' (get_x a)));
+    assert(forall (#t:Type) (b':buffer t). disjoint_from_bufs b' s
+	     ==> (disjoint b' (get_y a)));
+    assert(forall (#t:Type) (b':buffer t). disjoint_from_bufs b' s
+	     ==> (disjoint b' (get_z a)))
+
+#reset-options "--initial_fuel 0 --max_fuel 0 --z3timeout 100"
+
+val copy:
+  a:point{same_frame a} -> b:point{distinct a b} ->
+  Stack unit
+    (requires (fun h -> live h a /\ live h b))
+    (ensures (fun h0 _ h1 -> live h1 a /\ live h1 b
+      /\ HS.modifies_one (frame_of a) h0 h1
+      /\ HS.modifies_ref (frame_of a) (refs a) h0 h1
+      /\ prop_2 h0 h1 a))
+let copy a b =
+  let h0 = ST.get() in
+  blit (get_x b) 0ul (get_x a) 0ul nlength;
+  let h1 = ST.get() in
+  cut (live h1 a /\ live h1 b);
+  lemma_reveal_modifies_1 (get_x a) h0 h1;
+  blit (get_y b) 0ul (get_y a) 0ul nlength;
+  let h2 = ST.get() in
+  cut (live h2 a /\ live h2 b);
+  lemma_reveal_modifies_1 (get_y a) h1 h2;
+  blit (get_z b) 0ul (get_z a) 0ul nlength;
+  let h3 = ST.get() in
+  cut (live h2 a /\ live h2 b);
+  lemma_reveal_modifies_1 (get_z a) h2 h3;
+  helper_lemma' (get_x a);
+  helper_lemma' (get_y a);
+  helper_lemma' (get_z a);
+  helper_lemma_2 (frame_of a) h0 h1 !{as_ref (get_x a)} (refs a);
+  helper_lemma_2 (frame_of a) h1 h2 !{as_ref (get_y a)} (refs a);
+  helper_lemma_2 (frame_of a) h2 h3 !{as_ref (get_z a)} (refs a);
+  helper_lemma_3 (frame_of a) h0 h1 h2 (refs a);
+  helper_lemma_3 (frame_of a) h0 h2 h3 (refs a);
+  helper_lemma_4' (frame_of a) h0 h1 h2 h3 a;
+  assert(HS.modifies_ref (frame_of a) (refs a) h0 h3);
+  ()
+
+
+#reset-options "--initial_fuel 0 --max_fuel 0 --z3timeout 20"
+
+val swap:
+  a:point -> b:point{distinct a b /\ same_frame b} ->
+  Stack unit
+    (requires (fun h -> live h a /\ live h b))
+    (ensures (fun h0 _ h1 -> live h1 b /\ live h1 a
+      /\ HS.modifies_one (frame_of b) h0 h1
+      /\ HS.modifies_ref (frame_of b) (refs b) h0 h1
+      /\ prop_2 h0 h1 b ))
+let swap a b =
+  copy b a
+
+val helper_lemma_5: h0:mem -> h1:mem -> a:point -> b:point -> Lemma
+  (requires (prop_2 h0 h1 a /\ distinct a b /\ live h0 b /\ same_frame_2 a b))
+  (ensures  (live h1 b))
+let helper_lemma_5 h0 h1 a b =
+  let x = get_x b in
+  let y = get_y b in
+  let z = get_z b in
+  let s = (only (get_x a) ++ only (get_y a) ++ only (get_z a)) in
+  assert(disjoint_from_bufs x s);
+  assert(disjoint_from_bufs y s);
+  assert(disjoint_from_bufs z s)
+
+
+#reset-options "--initial_fuel 0 --max_fuel 0 --z3timeout 100"
+
+val swap_both:
+  a:point -> b:point{distinct a b /\ same_frame_2 a b} ->
+  c:point{distinct c a /\ distinct c b /\ same_frame_2 b c} ->
+  d:point{distinct d a /\ distinct d b /\ distinct d c /\ same_frame_2 c d} -> Stack unit
+    (requires (fun h -> live h a /\ live h b /\ live h c /\ live h d))
+    (ensures (fun h0 _ h1 -> live h1 a /\ live h1 b /\ live h1 c /\ live h1 d
+      /\ HS.modifies_one (frame_of a) h0 h1
+      /\ HS.modifies_ref (frame_of a) (refs a ++ refs b ++ refs c ++ refs d) h0 h1 ))
+let swap_both a b c d =
+  let h0 = ST.get() in
+  copy c a;
+  let h1 = ST.get() in
+  helper_lemma_5 h0 h1 c a;
+  helper_lemma_5 h0 h1 c b;
+  helper_lemma_5 h0 h1 c d;
+  copy d b;
+  let h2 = ST.get() in
+  helper_lemma_5 h1 h2 d a;
+  helper_lemma_5 h1 h2 d b;
+  helper_lemma_5 h1 h2 d c;
+  helper_lemma_2 (frame_of a) h0 h1 (refs c) (refs a ++ refs b ++ refs c ++ refs d);
+  helper_lemma_2 (frame_of a) h1 h2 (refs d) (refs a ++ refs b ++ refs c ++ refs d);
+  helper_lemma_3 (frame_of a) h0 h1 h2 (refs a ++ refs b ++ refs c ++ refs d);
+  ()
+
+
+#reset-options "--initial_fuel 0 --max_fuel 0 --z3timeout 100"
+
+val copy2: p':point -> q':point{distinct p' q' /\ same_frame_2 p' q'} ->
+  p:point{distinct p p' /\ distinct p q' /\ same_frame_2 p q'} ->
+  q:point{distinct q p' /\ distinct q q' /\ same_frame_2 p q} -> Stack unit
+    (requires (fun h -> live h p' /\ live h q' /\ live h p /\ live h q))
+    (ensures (fun h0 _ h1 -> live h1 p' /\ live h1 q' /\ live h1 p /\ live h1 q
+      /\ HS.modifies_one (frame_of p) h0 h1
+      /\ HS.modifies_ref (frame_of p) (refs p' ++ refs q') h0 h1 ))
+let copy2 p' q' p q =
+  let h0 = ST.get() in
+  copy p' p;
+  let h1 = ST.get() in
+  helper_lemma_5 h0 h1 p' q';
+  helper_lemma_5 h0 h1 p' p;
+  helper_lemma_5 h0 h1 p' q;
+  copy q' q;
+  let h2 = ST.get() in
+  helper_lemma_5 h1 h2 q' p';
+  helper_lemma_5 h1 h2 q' p;
+  helper_lemma_5 h1 h2 q' q;
+  helper_lemma_2 (frame_of p) h0 h1 (refs p') (refs p' ++ refs q');
+  helper_lemma_2 (frame_of p) h1 h2 (refs q') (refs p' ++ refs q');
+  helper_lemma_3 (frame_of p) h0 h1 h2 (refs p' ++ refs q');
+  ()
